\documentclass[preview]{standalone}
\usepackage{amssymb, amsthm}
\usepackage{mathtools}
\usepackage{bm}
\usepackage{xcolor}


\newtheorem*{theorem*}{Theorem}
\renewcommand\qedsymbol{$\blacksquare$}


\begin{document}


\begin{theorem*}[\textbf{2350}]
    Let \bm{$\zeta$} be a real number. 
    \begin{equation*}
        \bm{
            \lfloor - \zeta \rfloor 
                = 
            - \lceil \zeta \rceil
                \textbf{, and }
            \lceil - \zeta \rceil
                = 
            - \lfloor \zeta \rfloor
        }.
    \end{equation*}
\end{theorem*}

\begin{proof}
    By cases.
    \\ \\
    \bm{$(i)$} By the multiplicative compatibility laws from the order axioms,
    and by the properties for ceiling functions,
    there exists an integer \bm{$\lceil \zeta \rceil = \lambda$} such that
    \begin{equation*}
        \Bigg\{
            \Big \langle \lambda - 1 \Big \rangle
                <
            \Big \langle \zeta \Big \rangle
                \leq
            \Big \langle \lambda \Big \rangle
        \Bigg\}
            \equiv
        \Bigg\{
            \Big \langle - \lambda + 1 \Big \rangle 
                > 
            \Big \langle - \zeta \Big \rangle
                \ge 
            \Big \langle - \lambda \Big \rangle
        \Bigg\}
    \end{equation*}
    By the properties for floor functions, 
    \bm{$\lfloor - \zeta \rfloor = - \lambda$}.
    And \bm{$-1 \times \lceil \zeta \rceil = - \lambda$}, 
    by the multiplicative equality property for equations.
    Thus, \bm{$\lfloor - \zeta \rfloor = - \lceil \zeta \rceil$}, 
    by the identity \bm{$- \lambda$}.
    \\ \\
    \bm{$(ii)$} By the multiplicative compatibility laws from the order axioms,
    and by the properties of floor functions,
    there exists an integer \bm{$\lfloor \zeta \rfloor = \lambda$} such that
    \begin{equation*}
        \Bigg\{
            \Big \langle \lambda \Big \rangle
                \le 
            \Big \langle \zeta \Big \rangle
                < 
            \Big \langle \lambda + 1 \Big \rangle
        \Bigg\}
            \equiv
        \Bigg\{
            \Big \langle - \lambda \Big \rangle
                \ge 
            \Big \langle - \zeta \Big \rangle
                > 
            \Big \langle - \lambda - 1 \Big \rangle
        \Bigg\}
    \end{equation*}
    By the properties of ceiling functions,
    \bm{$\lceil - \zeta \rceil = - \lambda$}. 
    And  
    \bm{$- 1 \times \lfloor \zeta \rfloor = - \lambda$}, 
    by the multiplicative property for equations.
    Thus,
    \bm{$\lceil - \zeta \rceil = - \lfloor \zeta \rfloor$},
    by the identity \bm{$- \lambda$}.
    \\ \\
    $\therefore \text{\space}
    \bm{
            \lfloor - \zeta \rfloor 
                = 
            - \lceil \zeta \rceil
                \textbf{, and }
            \lceil - \zeta \rceil
                = 
            - \lfloor \zeta \rfloor
    }$.
\color{lightgray} \end{proof}

\end{document}