\documentclass[a4paper, 12pt]{article}
\usepackage[utf8]{inputenc}
\usepackage[english]{babel}
\usepackage{amssymb, amsmath, amsthm}
\theoremstyle{plain}
\newtheorem*{theorem*}{Theorem}
\newtheorem{theorem}{Theorem}

\usepackage{mathtools}
\renewcommand\qedsymbol{$\blacksquare$}

\begin{document}
	
	\begin{theorem*}[2.3.36a]
		Let f be the function $f: A \implies B$. Let S, and T be subsets of A. 
		$f(S \cup T) = f(S) \cup f(T)$.
	\end{theorem*}
	
	\begin{proof}
		By the definition for the image of a set $(S \cup T)$ under the function $f$ we have 
		$f(S \cup T) = \{t | \exists s \in S \cup T (t = f(s))\} 
		\equiv \{f(s) | s \in (S \cup T)\}$. Since $\{f(s) | s \in (S \cup T)\}$ is a set, from 
		this we can write $f(S \cup T) \equiv 
		\newline \{f(s) | (s \in S)\} \cup \{f(s) | (s \in T)\}$. The right-hand side of this 
		equivalence is the set $f(S) \cup f(T)$, by the definition for the image of a set $S$ or 
		$T$ under the function $f \therefore f(S \cup T) = f(S) \cup f(T)$.
	\end{proof}

\end{document}
