\documentclass[preview]{standalone}
\usepackage{amssymb, amsthm}
\usepackage{mathtools}
\usepackage{bm}


\newtheorem{theorem}{Theorem}
\renewcommand\qedsymbol{$\blacksquare$}


\begin{document}


\begin{theorem}[\textbf{2218d}]
    Let \bm{$\mathrm{A}$}, \bm{$\Lambda$}, and \bm{$\Delta$} be sets. 
    \bm{$
    \big \langle \mathrm{A} - \Delta \big \rangle
        \cap 
    \big \langle \Delta - \Lambda \big \rangle
        = 
    \varnothing
    $}.
\end{theorem}
\begin{proof}
    Let \bm{$\lambda$} be an element in 
    \bm{$
    \big \langle \mathrm{A} - \Delta \big \rangle
        \cap 
    \big \langle \Delta - \Lambda \big \rangle
    $}.
    By the definitions for set difference, and set intersection, that is
    \begin{equation*}
        \bigg[
            \Big \langle \lambda \in \mathrm{A} \Big \rangle
                \land
            \Big \langle \lambda \notin \Delta \Big \rangle
        \bigg]
            \land
        \bigg[
            \Big \langle \lambda \in \Delta \Big \rangle
                \land
            \Big \langle \lambda \notin \Lambda \Big \rangle
        \bigg]
    \end{equation*}
    Since logical conjunction is associative, 
    \bm{$\lambda$} is in \bm{$\Delta$},
    and \bm{$\lambda$} is not in \bm{$\Delta$}. 
    Thus, by the negation law of logic,
    \begin{equation*}
        \Big \langle \lambda \in \mathrm{A} \Big \rangle
            \land
        \Big \langle \bot \Big \rangle
            \land
        \Big \langle \lambda \notin \Lambda \Big \rangle
    \end{equation*}
    This statement is \bm{$\bot$}, 
    by the domination law for logical conjunction. 
    And the logical identity for \bm{$\lambda \in \varnothing$} is trivially \bm{$\bot$},
    since the empty set contains no members. 
    Hence,
    \begin{equation*}
        \bigg[
            \Big \langle \lambda \in \mathrm{A} \Big \rangle
                \land
            \Big \langle \lambda \notin \Delta \Big \rangle
        \bigg]
            \land
        \bigg[
            \Big \langle \lambda \in \Delta \Big \rangle
                \land
            \Big \langle \lambda \notin \Lambda \Big \rangle
        \bigg]
            \equiv
        \Big \langle \lambda \in \varnothing \Big \rangle
    \end{equation*}
    $\therefore \text{\space} \bm{
    \big \langle \mathrm{A} - \Delta \big \rangle
        \cap 
    \big \langle \Delta - \Lambda \big \rangle
        = 
    \varnothing
    }$,
    by the definitions for the difference of sets, 
    and for the intersection of sets.
\end{proof}


\end{document}