\documentclass[a4paper, 12pt]{article}
\usepackage[utf8]{inputenc}
\usepackage[english]{babel}
\usepackage{amssymb, amsmath, amsthm}
\theoremstyle{plain}
\newtheorem*{theorem*}{Theorem}
\newtheorem{theorem}{Theorem}

\usepackage{mathtools}
\renewcommand\qedsymbol{$\blacksquare$}
\DeclarePairedDelimiter{\floor}{\lfloor}{\rfloor}
\DeclarePairedDelimiter{\ceil}{\lceil}{\rceil}

\begin{document}
	
	\begin{theorem*}[2.4.21a]
		The summation of odd numbers from 1 to n is $n^{2}$.
	\end{theorem*}
	
	\begin{proof}
		$\sum_{k=1}^{n} 2k - 1 = \sum_{k=1}^{n} k^{2} - (k-1)^{2}$. By Theorem 2.4.19, that is \newline $n^{2} - 0^{2} = n^{2}$. Thus, $\sum_{k=1}^{n} 2k - 1 = n^{2}$, and indeed the summation of odd numbers from $1$ to $n$ is $n^{2}$.
	\end{proof}

\end{document}
