\documentclass[a4paper, 12pt]{article}
\usepackage[utf8]{inputenc}
\usepackage[english]{babel}
\usepackage{amssymb, amsmath, amsthm}
\theoremstyle{plain}
\newtheorem*{theorem*}{Theorem}
\newtheorem{theorem}{Theorem}

\usepackage{mathtools}
\renewcommand\qedsymbol{$\blacksquare$}

\begin{document}
	
	\begin{theorem*}[2.2.18d]
		Let A, B, and C be sets. $(A - C) \cap (C - B) = \emptyset$.
	\end{theorem*}
	
	\begin{proof}
		Let $x$ be an element in $(A - C) \cap (C - B)$. This is equivalently stated as 
		$x \in [(A \cap \overline{C}) \cap (C \cap \overline{B})]$. Since set intersection is 
		associative the inner parentheses can be eliminated, 
		$x \in (A \cap \overline{C} \cap C \cap \overline{B})$. An expression the definition for which 
		is $(x \in A) \land (x \in \overline{C}) \land (x \in C) \land (x \in \overline{B})$. But by the 
		logical law of negation this definition states 
		$(x \in A) \land \bot \land (x \in \overline{B}) \equiv \bot$. Meaning 
		$\lnot \exists x (x \in (A - C) \cap (C - B))$. In other words, the intersection is indeed empty.
	\end{proof}

\end{document}
