\documentclass[preview]{standalone}
\usepackage{amssymb, amsthm}
\usepackage{mathtools}
\usepackage{bm}


\newtheorem{theorem}{Theorem}
\renewcommand\qedsymbol{$\blacksquare$}


\begin{document}


\begin{theorem}[\textbf{2367c}]
    Let \bm{$\Lambda$} be a set with universal set \bm{$\Omega$}.
    \\
    Let \bm{$\lambda_{\overline{\Lambda}}$} be the characteristic function 
    \bm{$\lambda_{\overline{\Lambda}}: \Omega \rightarrow \{0, 1\}$}. 
    \begin{equation*}
        \bm{
            \lambda_{\overline{\Lambda}} \big[ \iota \big] 
                = 
            1 - \lambda_{\Lambda} \big[ \iota \big]
        }
    \end{equation*}
\end{theorem}

\begin{proof}
    By cases. There are two cases. 
    Either $(i)$ \bm{$\iota$} is in \bm{$\Lambda$},
    xor $(ii)$ \bm{$\iota$} is in \bm{$\overline{\Lambda}$}.
    \\ \\
    \bm{$(i)$} Let \bm{$\iota$} be an element in \bm{$\Lambda$}. 
    By the double negation law, 
    by the definition for set membership,
    by the definition for set complement,
    and again by the defintion for set membership, that is
    \begin{equation*}
        \lnot \bigg[ \lnot \Big \langle \iota \in \Lambda \Big \rangle \bigg]
            \equiv
        \lnot \Big \langle \iota \notin \Lambda \Big \rangle
            \equiv
        \lnot \Big \langle \iota \in \overline{\Lambda} \Big \rangle
            \equiv
        \Big \langle \iota \notin \overline{\Lambda} \Big \rangle
    \end{equation*}
    Thus, by the definition for characteristic functions 
    \begin{equation*}
        \Big \langle 
            \lambda_{\overline{\Lambda}} \big[ \iota \big] = 0
        \Big \rangle
            \land
        \Big \langle 
            \lambda_{\Lambda} \big[ \iota \big] = 1
        \Big \rangle
    \end{equation*}
    $\therefore \text{\space} \bm{
        \lambda_{\overline{\Lambda}} \big[ \iota \big] 
            = 
        1 - \lambda_{\Lambda} \big[ \iota \big]
    }$.
    \\ \\
    \bm{$(ii)$} Let \bm{$\iota$} be an element in \bm{$\overline{\Lambda}}$.
    By the double negation law, 
    by the definition for set membership,
    by the definition for set complement,
    and again by the defintion for set membership, that is
    \begin{equation*}
        \lnot \bigg[ \lnot \Big \langle \iota \in \overline{\Lambda} \Big \rangle \bigg]
            \equiv
        \lnot \Big \langle \iota \notin \overline{\Lambda} \Big \rangle
            \equiv
        \lnot \Big \langle \iota \in \Lambda \Big \rangle
            \equiv
        \Big \langle \iota \notin \Lambda \Big \rangle
    \end{equation*}
    Thus, by the definition for characteristic functions 
    \begin{equation*}
        \Big \langle 
            \lambda_{\overline{\Lambda}} \big[ \iota \big] = 1
        \Big \rangle
            \land
        \Big \langle 
            \lambda_{\Lambda} \big[ \iota \big] = 0
        \Big \rangle
    \end{equation*}
    $\therefore \text{\space} \bm{
        \lambda_{\overline{\Lambda}} \big[ \iota \big] 
            = 
        1 - \lambda_{\Lambda} \big[ \iota \big]
    }$.
\end{proof}


\end{document}