\documentclass[a4paper, 12pt]{article}
\usepackage[utf8]{inputenc}
\usepackage[english]{babel}
\usepackage{amssymb, amsmath, amsthm}
\theoremstyle{plain}
\newtheorem*{theorem*}{Theorem}
\newtheorem{theorem}{Theorem}

\usepackage{mathtools}
\renewcommand\qedsymbol{$\blacksquare$}
\DeclarePairedDelimiter{\floor}{\lfloor}{\rfloor}
\DeclarePairedDelimiter{\ceil}{\lceil}{\rceil}

\begin{document}
	
	\begin{theorem*}[2.3.44]
		Let x be a real number. $\ceil{x} - \floor{x} = 1$, if $x \notin \mathbb{Z}$. \newline 
		$\ceil{x} - \floor{x} = 0$, if $x \in \mathbb{Z}$. 
	\end{theorem*}
	
	\begin{proof}
		By cases. \newline \newline
		$(i)$ Suppose $x \notin \mathbb{Z}$. $\ceil{x} = \floor{x} + 1$. Thus, 
		$\ceil{x} - \floor{x} = (\floor{x} + 1) - \floor{x} = 1$. \newline \newline 
		$(ii)$ Suppose $x \in \mathbb{Z}$. $\ceil{x} = \floor{x} = x$. Thus, 
		$\ceil{x} - \floor{x} = x - x = 0$.
	\end{proof}

\end{document}
