\documentclass[preview]{standalone}
\usepackage{amssymb, amsthm}
\usepackage{mathtools}
\usepackage{bm}
\usepackage{xcolor}


\newtheorem*{theorem*}{Theorem}
\renewcommand\qedsymbol{$\blacksquare$}


\begin{document}


\begin{theorem*}[\textbf{2348a}]
    Let \bm{$\lambda$} be a real number, 
    and let \bm{$\zeta$} be an integer.
    \begin{equation*}
        \bm{
        \big \langle \lambda \le \zeta \big \rangle
            \textbf{ if and only if } 
        \big \langle \lceil \lambda \rceil \le \zeta \big \rangle
        }
    \end{equation*}
\end{theorem*}

\begin{proof}
    Direct form by the contrapositive. 
    Assume the negation of the direct consequent,
    such that \bm{$\lceil \lambda \rceil > \zeta$}. 
    By Theorem 2347b, 
    \bm{$\lambda > \zeta$}.
    Thus,
    \begin{equation*}
        \bigg[
            \Big \langle \lambda \Big \rangle
                \leq 
            \Big \langle \zeta \Big \rangle
        \bigg]
            \rightarrow 
        \bigg[
            \Big \langle \lceil \lambda \rceil \Big \rangle
                \leq 
            \Big \langle \zeta \Big \rangle
        \bigg]
    \end{equation*}
    Converse form by the contrapositive. 
    Assume the negation of the direct hypothesis, 
    such that \bm{$\lambda > \zeta$}.
    By Theorem 2347b, \bm{$\lceil \lambda \rceil > \zeta$}. 
    Thus,
    \begin{equation*}
        \bigg[
            \Big \langle \lceil \lambda \rceil \Big \rangle
                \leq 
            \Big \langle \zeta \Big \rangle
        \bigg]
            \rightarrow 
        \bigg[
            \Big \langle \lambda \Big \rangle
                \leq 
            \Big \langle \zeta \Big \rangle
        \bigg]
    \end{equation*}
    $\therefore \text{\space} \bm{
        \big \langle \lambda \le \zeta \big \rangle
            \textbf{ \emph{if and only if} } 
        \big \langle \lceil \lambda \rceil \le \zeta \big \rangle}
    $.
\color{lightgray} \end{proof}

\end{document}