\documentclass[preview]{standalone}
\usepackage{amssymb, amsthm}
\usepackage{mathtools}
\usepackage{bm}
\usepackage{xcolor}


\newtheorem*{theorem*}{Theorem}
\renewcommand\qedsymbol{$\blacksquare$}


\begin{document}


\begin{theorem*}[\textbf{2329a}]
    Let \bm{$\lambda$} be a function 
    \bm{$\lambda: \Delta \rightarrow \mathrm{A}$}, 
    and let \bm{$\epsilon$} be a function 
    \bm{$\epsilon: \Lambda \rightarrow \Delta$}. 
    If both \bm{$\lambda$} and \bm{$\epsilon$} are injective, 
    then \bm{$\big \langle \lambda \circ \epsilon \big \rangle$} is injective.
\end{theorem*}

\begin{proof}
    By the contrapositive.
    Suppose it were not the case that 
    \bm{$\big \langle \lambda \circ \epsilon \big \rangle$}
    were injective. 
    By the definition for injective functions, 
    with domain of discourse 
    \bm{$\big \langle \iota, \zeta \in \Lambda \big \rangle$}, that is
    \begin{equation*}
        \lnot \forall \iota \forall \zeta \bigg \langle 
            \Big[
                \big \langle \lambda \circ \epsilon \big \rangle [\iota] 
                    = 
                \big \langle \lambda \circ \epsilon \big \rangle [\zeta] 
            \Big]
                \rightarrow 
            \big \langle \iota = \zeta \big \rangle 
        \bigg \rangle
    \end{equation*}
    The composition of functions 
    \bm{$\big \langle \lambda \circ \epsilon \big \rangle [\iota]$} 
    is defined as \bm{$\lambda \big[ \epsilon (\iota) \big]$}. 
    Thus, we have the equivalent universal quantification
    \begin{equation*}
        \lnot \forall \iota \forall \zeta \bigg \langle 
            \Big[
                \lambda \big[ \epsilon (\iota) \big] 
                    = 
                \lambda \big[ \epsilon (\zeta) \big] 
            \Big]
                \rightarrow
            \big \langle \iota = \zeta \big \rangle
        \bigg \rangle
    \end{equation*}
    In other words, it follows from the negation of the direct consequent that 
    it is not the case that \bm{$\lambda$} is injective, 
    by the definition for injective functions. 
    This is sufficient to prove the logical negation of the direct hypothesis. 
    Thus, if both \bm{$\lambda$} and \bm{$\epsilon$} are injective, 
    then 
    \bm{$\big \langle \lambda \circ \epsilon \big \rangle$} 
    is injective.
\color{lightgray} \end{proof}

\end{document}