\documentclass[a4paper, 12pt]{article}
\usepackage[utf8]{inputenc}
\usepackage[english]{babel}
\usepackage{amssymb, amsmath, amsthm}
\theoremstyle{plain}
\newtheorem*{theorem*}{Theorem}
\newtheorem{theorem}{Theorem}

\usepackage{mathtools}
\renewcommand\qedsymbol{$\blacksquare$}
\DeclarePairedDelimiter{\floor}{\lfloor}{\rfloor}
\DeclarePairedDelimiter{\ceil}{\lceil}{\rceil}

\begin{document}
	
	\begin{theorem*}[2.4.20]
		$\sum_{k=1}^{n} \frac{1}{k(k+1)} = \frac{n}{n+1}$.
	\end{theorem*}
	
	\begin{proof}
		$\sum_{k=1}^{n} \frac{1}{k(k+1)} = \sum_{k=1}^{n} (\frac{1}{k} - \frac{1}{k+1})$ = \newline
		$(\frac{1}{n} - \frac{1}{n+1}) + (\frac{1}{n-1} - \frac{1}{n}) + 
		(\frac{1}{n-2} - \frac{1}{n-1}) + \dots + 
		(\frac{1}{1} - \frac{1}{2})
		$ By Theorem 2.4.19, that is, $-\frac{1}{n+1} + \frac{1}{1} = \frac{(-1) + (n+1)}{n+1} = \frac{n}{n+1}$.
	\end{proof}

\end{document}
