\documentclass[preview]{standalone}
\usepackage{amssymb, amsthm}
\usepackage{mathtools}
\usepackage{bm}


\newtheorem{theorem}{Theorem}
\renewcommand\qedsymbol{$\blacksquare$}


\begin{document}


\begin{theorem}[\textbf{2216e}]
    Let \bm{$\mathrm{A}$} and \bm{$\Lambda$} be sets. 
    \bm{$
    \mathrm{A} 
        \cup 
    \big \langle \Lambda - \mathrm{A} \big \rangle 
        = 
    \mathrm{A} \cup \Lambda
    $}.
\end{theorem}
\begin{proof}
    Let \bm{$\lambda$} be an element in 
    \bm{$\mathrm{A} \cup \big \langle \Lambda - \mathrm{A} \big \rangle$}. 
    By the definitions for set difference, and set union, that is
    \begin{equation*}
        \Big \langle \lambda \in \mathrm{A} \Big \rangle 
            \lor 
        \bigg[
            \Big \langle \lambda \in \Lambda \Big \rangle 
                \land 
            \Big \langle \lambda \notin \mathrm{A} \Big \rangle 
        \bigg] 
    \end{equation*}
    Distributing the logical disjunction over logical conjunction yields
    \begin{equation*}
        \bigg[
            \Big \langle \lambda \in \mathrm{A} \Big \rangle 
                \lor 
            \Big \langle \lambda \in \Lambda \Big \rangle
        \bigg]
            \land
        \bigg[
            \Big \langle \lambda \in \mathrm{A} \Big \rangle
                \lor
            \Big \langle \lambda \notin \mathrm{A} \Big \rangle 
        \bigg]
    \end{equation*} 
    By the negation law for logical disjunction, 
    and by the identity law for logical conjunction, that is
    \begin{equation*}
        \Big \langle \lambda \in \mathrm{A} \Big \rangle 
        \lor 
        \Big \langle \lambda \in \Lambda \Big \rangle
    \end{equation*}
    Thus, 
    \begin{equation*}
        \Big \langle \lambda \in \mathrm{A} \Big \rangle 
            \lor 
        \bigg[
            \Big \langle \lambda \in \Lambda \Big \rangle 
                \land 
            \Big \langle \lambda \notin \mathrm{A} \Big \rangle 
        \bigg]
        \equiv
        \Big \langle \lambda \in \mathrm{A} \Big \rangle 
            \lor 
        \Big \langle \lambda \in \Lambda \Big \rangle\
    \end{equation*}
    $\therefore$ by the definition of set union,
    \bm{$
    \mathrm{A} 
        \cup 
    \big \langle \Lambda - \mathrm{A} \big \rangle 
        = 
    \mathrm{A} \cup \Lambda
    $}.
\end{proof}


\end{document}