\documentclass[preview]{standalone}
\usepackage{amssymb, amsthm}
\usepackage{mathtools}
\usepackage{bm}
\usepackage{xcolor}


\newtheorem*{theorem*}{Theorem}
\renewcommand\qedsymbol{$\blacksquare$}


\begin{document}


\begin{theorem*}[\textbf{2218e}] \color{black}
    Let \bm{$\mathrm{A}$}, \bm{$\Lambda$}, and \bm{$\Delta$} be sets. 
    \bm{$
    \big \langle \Lambda - \mathrm{A} \big \rangle 
        \cup 
    \big \langle \Delta - \mathrm{A} \big \rangle 
        = 
    \big \langle \Lambda \cup \Delta \big \rangle - \mathrm{A}
    $}.
\end{theorem*}
\begin{proof} \color{black}
    Let \bm{$\lambda$} be an element in 
    \bm{$
    \big \langle \Lambda - \mathrm{A} \big \rangle 
        \cup 
    \big \langle \Delta - \mathrm{A} \big \rangle
    $}.
    By the definitions for set difference, and the union of sets, that is
    \begin{equation*}
        \bigg[
            \Big \langle \lambda \in \Lambda \Big \rangle
                \land
            \Big \langle \lambda \notin \mathrm{A} \Big \rangle
        \bigg]
            \lor
        \bigg[
            \Big \langle \lambda \in \Delta \Big \rangle
                \land
            \Big \langle \lambda \notin \mathrm{A} \Big \rangle
        \bigg]
    \end{equation*}
    Factoring \bm{$\lambda \notin \mathrm{A}$} out, 
    by the distributive laws for logical conjunction over disjunction,
    \begin{equation*}
        \Bigg\{
            \bigg[
                \Big \langle \lambda \in \Lambda \Big \rangle
                    \land
                \Big \langle \lambda \notin \mathrm{A} \Big \rangle
            \bigg]
                \lor
            \bigg[
                \Big \langle \lambda \in \Delta \Big \rangle
                    \land
                \Big \langle \lambda \notin \mathrm{A} \Big \rangle
            \bigg]
        \Bigg\}
            \equiv
    \end{equation*}
    \begin{equation*}
        \Bigg\{
            \bigg[
                \Big \langle \lambda \in \Lambda \Big \rangle
                    \lor
                \Big \langle \lambda \in \Delta \Big \rangle
            \bigg]
                \land
            \Big \langle \lambda \notin \mathrm{A} \Big \rangle
        \Bigg\}
    \end{equation*}
    $\therefore \text{\space} \bm{
    \big \langle \Lambda - \mathrm{A} \big \rangle 
        \cup 
    \big \langle \Delta - \mathrm{A} \big \rangle 
        = 
    \big \langle \Lambda \cup \Delta \big \rangle - \mathrm{A}
    }$,
    by the defintions for set difference, and set union.
\color{lightgray} \end{proof}

\end{document}