\documentclass[a4paper, 12pt]{article}
\usepackage[utf8]{inputenc}
\usepackage[english]{babel}
\usepackage{amssymb, amsmath, amsthm}
\theoremstyle{plain}
\newtheorem*{theorem*}{Theorem}
\newtheorem{theorem}{Theorem}

\usepackage{mathtools}
\renewcommand\qedsymbol{$\blacksquare$}
\DeclarePairedDelimiter{\floor}{\lfloor}{\rfloor}
\DeclarePairedDelimiter{\ceil}{\lceil}{\rceil}

\begin{document}
	
\begin{theorem*}[\textbf{2.4.22}]
    The sum of squares from 1 to n is $$\frac{n(n+1)(2n+1)}{6}$$.
\end{theorem*}

\begin{proof}
    Let $\{a_n\}$ be the sequence of integers from $1$ to $n$. The formula for the 
    summation of squares from $1$ to $n$ can be derived from the cube of $n$. By 
    theorem 2.4.19, $$n^3 = \sum_{k=1}^{n} k^3 - (k-1)^3$$ This summation is 
    telescopic, and thus collapses to $n^3 - (1 - 1)^3 = n^3$. The expansion for 
    $(k-1)^3$ in that term of summation is $k^{3} - 3k^{2} + 3k - 1$, by the Binomial 
    Theorem. Thus, yielding the algebraic identity 
    $$k^{3} - (k - 1)^{3} = 3k^{2} - 3k + 1$$ Hence, 
    $n^{3} = \sum_{k=1}^{n} 3k^{2} - 3k + 1$, and by the field axioms,
    $$n^{3} = \left(3\sum_{k=1}^{n} k^{2}\right) - \left(3\sum_{k=1}^{n} k\right) + \left(\sum_{k=1}^{n} 1\right)$$
    Note that $(\sum_{k=1}^n 1) = n(1)$, and by Theorem 2.4.21b, 
    $(3\sum_{k=1}^{n} k) = 3(\frac{n(n+1)}{2})$. Thus, 
    $$n^{3} + 3\frac{n(n+1)}{2} - n = 3\sum_{k=1}^{n} k^{2}$$
    Eliminating the coefficient 
    $3$ from the right-hand side by division gives us the sum of squares in terms of an 
    equation, $$\frac{1}{3}\left(n^{3} + 3\frac{n(n+1)}{2} - n\right) = \sum_{k=1}^{n} k^{2}$$ 
    All that is left to do is to simplify the left-hand side 
    $\frac{1}{3}[n^{3} + 3\frac{n(n+1)}{2} - n] = \frac{2n^{3} + 3n^{2} + 3n - 2n}{6}$. 
    Factoring $\frac{1}{6}n$ gives 
    $\frac{1}{6}n(2n^{2} + 3n + 3 - 2) = \frac{1}{6}n(2n^{2} + 2n + n + 1)$. Factoring $2n$
    out of the first two terms in the sum, $\frac{1}{6}n[2n(n + 1) + (n + 1)]$. The 
    simplification process is complete by factoring $(n+1)$ out of the sum, \\ 
    $\frac{1}{6}n(n+1)(2n+1)$. Thus, the sum of squares $$\sum_{k=1}^{n} k^{2} = 
    \frac{n(n+1)(2n+1)}{6}$$
\end{proof}

\end{document}
