\documentclass[preview]{standalone}
\usepackage{amssymb, amsthm}
\usepackage{mathtools}
\usepackage{bm}
\usepackage{xcolor}


\newtheorem*{theorem*}{Theorem}
\renewcommand\qedsymbol{$\blacksquare$}


\begin{document}


\begin{theorem*}[\textbf{2336a}]
    Let \bm{$\lambda$} be the function 
    \bm{$\lambda: \Gamma \to \Phi$}. 
    Let \bm{$\mathrm{A}$}, and \bm{$\Lambda$} be subsets of \bm{$\Gamma$}. 
    \begin{equation*}
        \bm{
            \lambda \big[ \mathrm{A} \cup \Lambda \big] 
                = 
            \lambda \big[ \mathrm{A} \big] \cup \lambda \big[ \Lambda \big]
        }
    \end{equation*}
\end{theorem*}

\begin{proof}
    Suppose there exists an element \bm{$\phi$} such that
    \bm{$\phi \in \lambda \big[ \mathrm{A} \cup \Lambda \big]$}.
    By the definition for the image of a set under the function \bm{$\lambda$},
    \bm{$\phi = \lambda \big[ \iota \big]$} 
    where \bm{$\iota$} is an element in \bm{$\mathrm{A} \cup \Lambda$}. 
    That is, by the definition for the union of sets,
    \bm{$\iota \in \mathrm{A} \lor \iota \in \Lambda$}. 
    Thus, 
    \bm{$\phi \in \lambda \big[ \mathrm{A} \big] \lor \phi \in \lambda \big[ \Lambda \big]$}.
    And by the definition for set union, 
    \bm{$\phi \in \lambda \big[ \mathrm{A} \big] \cup \lambda \big[ \Lambda \big]$}.
    
    Suppose there exists an element \bm{$\phi$} such that 
    \bm{$\phi \in \lambda \big[ \mathrm{A} \big] \cup \lambda \big[ \Lambda \big]$}.
    By the defintion for set union, 
    \bm{$\phi \in \lambda \big[ \mathrm{A} \big] \lor \phi \in \lambda \big[ \Lambda \big]$}.
    By the definition for the image of a set under the function \bm{$\lambda$},
    there exists an element \bm{$\iota \in \mathrm{A} \lor \iota \in \Lambda$} such that 
    \bm{$\lambda \big[ \iota \big] = \phi$}.
    By the definition for set union, 
    \bm{$\iota \in \mathrm{A} \cup \Lambda$}.
    Hence,
    \bm{$\phi \in \lambda \big[ \mathrm{A} \cup \Lambda \big]$}
\color{lightgray} \end{proof}

\end{document}