\documentclass[preview]{standalone}
\usepackage{amssymb, amsthm}
\usepackage{mathtools}
\usepackage{bm}


\newtheorem{theorem}{Theorem}
\renewcommand\qedsymbol{$\blacksquare$}


\begin{document}


\begin{theorem}[\textbf{2348b}]
    Let \bm{$\lambda$} be a real number, 
    and let \bm{$\zeta$} be an integer. 
    \begin{equation*}
        \bm{
        \big \langle \zeta \le \lambda \big \rangle
            \textbf{ if and only if }
        \big \langle \zeta \le \lfloor \lambda \rfloor \big \rangle}
    \end{equation*}
\end{theorem}

\begin{proof}
    Direct form by the contrapositive.
    Assume the negation of the direct consequent,
    such that \bm{$\zeta > \lfloor \lambda \rfloor$}.
    By Theorem 79, \bm{$\zeta > \lambda$}.
    Thus,
    \begin{equation*}
        \bigg[
            \Big \langle \zeta \Big \rangle
                \leq 
            \Big \langle \lambda \Big \rangle
        \bigg]
            \rightarrow 
        \bigg[
            \Big \langle \zeta \Big \rangle
                \leq 
            \Big \langle \lfloor \lambda \rfloor \Big \rangle
        \bigg]
    \end{equation*}
    Converse form by the contrapositive.
    Assume the negation of the direct hypothesis,
    such that \bm{$\zeta > \lambda$}.
    By Theorem 79, 
    \bm{$\zeta > \lfloor \lambda \rfloor$}.
    Thus,
    \begin{equation*}
        \bigg[
            \Big \langle \zeta \Big \rangle
                \leq 
            \Big \langle \lfloor \lambda \rfloor \Big \rangle
        \bigg]
            \rightarrow 
        \bigg[
            \Big \langle \zeta \Big \rangle
                \leq 
            \Big \langle \lambda \Big \rangle
        \bigg]
    \end{equation*}
    $\therefore \text{\space} \bm{
        \big \langle \zeta \le \lambda \big \rangle
            \textbf{ \emph{if and only if} }
        \big \langle \zeta \le \lfloor \lambda \rfloor \big \rangle}
    $.
\end{proof}


\end{document}