\documentclass[a4paper, 12pt]{article}
\usepackage[utf8]{inputenc}
\usepackage[english]{babel}
\usepackage{amssymb, amsmath, amsthm}
\theoremstyle{plain}
\newtheorem*{theorem*}{Theorem}
\newtheorem{theorem}{Theorem}

\usepackage{mathtools}
\renewcommand\qedsymbol{$\blacksquare$}
\DeclarePairedDelimiter{\floor}{\lfloor}{\rfloor}
\DeclarePairedDelimiter{\ceil}{\lceil}{\rceil}

\begin{document}
	
	\begin{theorem*}[2.4.21b]
		The summation of natural numbers from 1 to n is $\frac{n(n+1)}{2}$.
	\end{theorem*}
	
	\begin{proof}
		By Theorem 2.4.21a we know that $\sum_{k=1}^{n} 2k - 1 = n^{2}$. This is the same as saying $-n + \sum_{k=1}^{n} 2k = n^{2} \equiv \sum_{k=1}^{n} 2k = n^{2} + n = n(n + 1)$. We can factor the coefficient $2$ out of the term of summation, $2 \sum_{k=1}^{n} k = n(n+1)$. And of course dividing both sides by $2$ gives $\sum_{k=1}^{n} k = \frac{n(n+1)}{2}$. Thus, indeed, the summation of natural numbers from 1 to n is $\frac{n(n+1)}{2}$.
	\end{proof}

\end{document}
