\documentclass[a4paper, 12pt]{article}
\usepackage[utf8]{inputenc}
\usepackage[english]{babel}
\usepackage{amssymb, amsmath, amsthm}
\theoremstyle{plain}
\newtheorem*{theorem*}{Theorem}
\newtheorem{theorem}{Theorem}

\usepackage{mathtools}
\renewcommand\qedsymbol{$\blacksquare$}
\DeclarePairedDelimiter{\floor}{\lfloor}{\rfloor}
\DeclarePairedDelimiter{\ceil}{\lceil}{\rceil}

\begin{document}
	
\begin{theorem*}[\textbf{2.4.20}]
    $$\sum_{k=1}^{n} \frac{1}{k(k+1)} = \frac{n}{n+1}$$
\end{theorem*}

\begin{proof}
    The identity of $\left(\frac{1}{k(k+1)}\right)$ is 
    $\left(\frac{1}{k} - \frac{1}{(k+1)}\right)$. This can be 
    demonstrated by the equation  
    $$k\left(\frac{1}{k} - \frac{1}{(k+1)}\right) = \left(\frac{k+1}{k+1} - \frac{k}{k+1}\right)
    = \left(\frac{k + 1 - k}{k+1}\right) = \left(\frac{1}{k+1}\right)$$ Dividing both sides of this equation by $k$ gives the desired
    identity such that
    $$\sum_{k=1}^n \frac{1}{k(k+1)} = \sum_{k=1}^{n} \left(\frac{1}{k} - \frac{1}{k+1}\right)$$
    The sequence for which is the telescopic summation
    $$\left(\frac{1}{n} - \frac{1}{n+1}\right) + \left(\frac{1}{n-1} - \frac{1}{n}\right) + 
    \left(\frac{1}{n-2} - \frac{1}{n-1}\right) + \dots + \left(\frac{1}{1} - \frac{1}{2}\right)$$ 
    Thus, by Theorem 2.4.19
    $$\sum_{k=1}^{n} \frac{1}{k(k+1)} = \left(-\frac{1}{n+1} + \frac{1}{1}\right) = \left(\frac{(-1) + (n+1)}{n+1}\right) = \frac{n}{n+1}$$
\end{proof}

\end{document}
