\documentclass[preview]{standalone}
\usepackage{amssymb, amsthm}
\usepackage{mathtools}
\usepackage{bm}


\newtheorem{theorem}{Theorem}
\renewcommand\qedsymbol{$\blacksquare$}


\begin{document}


\begin{theorem}[\textbf{2218c}]
    Let \bm{$\mathrm{A}$}, \bm{$\Lambda$}, and \bm{$\Delta$} be sets. 
    \bm{$
    \big \langle \mathrm{A} - \Lambda \big \rangle - \Delta 
        \subseteq 
    \big \langle \mathrm{A} - \Delta \big \rangle
    $}.
\end{theorem}
\begin{proof}
    Let \bm{$\lambda$} be an element in 
    \bm{$\big \langle \mathrm{A} - \Lambda \big \rangle - \Delta$}. 
    By the definition for set difference, that is
    \begin{equation*}
        \bigg[
            \Big \langle \lambda \in \mathrm{A} \Big \rangle
                \land
            \Big \langle \lambda \notin \Lambda \Big \rangle
        \bigg]
            \land
        \Big \langle \lambda \notin \Delta \Big \rangle
    \end{equation*}
    By the law of associativity for logical conjunction, 
    by the law of commutativity for logical conjunction,
    and by the simplification rule of inference,
    \begin{equation*}
        \Bigg\{
            \bigg[
                \Big \langle \lambda \in \mathrm{A} \Big \rangle
                    \land
                \Big \langle \lambda \notin \Lambda \Big \rangle
            \bigg]
                \land
            \Big \langle \lambda \notin \Delta \Big \rangle
        \Bigg\}
            \equiv
        \Bigg\{
            \bigg[
                \Big \langle \lambda \in \mathrm{A} \Big \rangle
                    \land
                \Big \langle \lambda \notin \Delta \Big \rangle
            \bigg]
                \land
            \Big \langle \lambda \notin \Lambda \Big \rangle
        \Bigg\}
    \end{equation*}
    \begin{equation*}
            \to
        \Big \langle \lambda \in \mathrm{A} \Big \rangle
            \land
        \Big \langle \lambda \notin \Delta \Big \rangle
    \end{equation*}
    $\therefore \text{\space} \bm{
    \big \langle \mathrm{A} - \Lambda \big \rangle - \Delta 
        \subseteq 
    \big \langle \mathrm{A} - \Delta \big \rangle
    }$,
    by the definitions for set difference and subsets.
\end{proof}


\end{document}