\documentclass[preview]{standalone}
\usepackage{amssymb, amsthm}
\usepackage{mathtools}
\usepackage{bm}
\usepackage{xcolor}


\newtheorem*{theorem*}{Theorem}
\renewcommand\qedsymbol{$\blacksquare$}


\begin{document}


\begin{theorem*}[\textbf{2340b}]
    Let \bm{$\lambda$} be the function 
    \bm{$\lambda : \Gamma \rightarrow \mathrm{A}$}. 
    Let \bm{$\Lambda$}, and \bm{$\Delta$} 
    be subsets of \bm{$\mathrm{A}$}. 
    \begin{equation*}
        \bm{
        \lambda ^{-1} \big[ \Lambda \cap \Delta \big] 
            = 
        \lambda ^{-1} 
            \big[ \Lambda \big] 
                \cap 
            \lambda^{-1} \big[ \Delta \big]
        }
    \end{equation*}
\end{theorem*}

\begin{proof}
    Let \bm{$\iota$} be an element in \bm{$\lambda ^{-1} \big[ \Lambda \cap \Delta \big]$}.
    By the inverse function for
    \bm{$\lambda ^{-1}$}, 
    and by the definition for the intersection of sets, that is 
    \begin{equation*}
        \bigg \langle \lambda 
            \big[ \iota \big] 
                \in 
            \lambda \Big[ 
                \lambda ^{-1} \big[ \Lambda \cap \Delta \big]
            \Big]
        \bigg \rangle
            \equiv
        \bigg[
            \Big \langle \lambda \big[ \iota \big] \in \Lambda \Big \rangle
                \land 
            \Big \langle \lambda \big[ \iota \big] \in \Delta \Big \rangle
        \bigg]
    \end{equation*}
    By \bm{$\lambda$} inverse, and by the definition for set intersection, that is
    \begin{equation*}
        \bigg[
            \Big \langle
                \iota \in \lambda^{-1} \big[ \Lambda \big] 
            \Big \rangle
                \land 
            \Big \langle
                \iota \in \lambda^{-1} \big[ \Delta \big]
            \Big \rangle
        \bigg]
            \equiv
        \bigg[ 
            \iota \in \Big \langle
                \lambda ^{-1} \big[ \Lambda \big] 
                    \cap 
                \lambda ^{-1} \big[ \Delta \big]
            \Big \rangle
        \bigg]
    \end{equation*}
    $\therefore \text{\space} \bm{
    \lambda ^{-1} \big[ \Lambda \cap \Delta \big] 
        = 
    \lambda ^{-1} 
        \big[ \Lambda \big] 
            \cap 
        \lambda^{-1} \big[ \Delta \big]
    }$.
\color{lightgray} \end{proof}

\end{document}