\documentclass[preview]{standalone}
\usepackage{amssymb, amsthm}
\usepackage{mathtools}
\usepackage{bm}
\usepackage{xcolor}


\newtheorem*{theorem*}{Theorem}
\renewcommand\qedsymbol{$\blacksquare$}


\begin{document}


\begin{theorem*}[\textbf{2217}] \color{black}
    Let \bm{$\mathrm{A}$}, \bm{$\Lambda$}, and \bm{$\Delta$} be sets. 
    \bm{$
    \overline{
            \mathrm{A} 
                \cap 
            \Lambda 
                \cap 
            \Delta
    } 
        = 
    \overline{\mathrm{A}} 
        \cup 
    \overline{\Lambda} 
        \cup 
    \overline {\Delta}
    $}.
\end{theorem*}
\begin{proof} \color{black}
    Let \bm{$\lambda$} be an element in 
    \bm{$\overline{\mathrm{A} \cap \Lambda \cap \Delta}$}. 
    By the definitions for set complementation and set membership, that is
    \begin{equation*}
        \lambda \notin \mathrm{A} \cap \Lambda \cap \Delta 
            \equiv 
        \lnot \big[ \lambda \in
            \mathrm{A} \cap \Lambda \cap \Delta
        \big]
    \end{equation*}
    The following statement is equivalent, by the definition for set intersection,
    \begin{equation*}
        \lnot \Big[
            \big \langle \lambda \in \mathrm{A} \big \rangle 
                \land 
            \big \langle \lambda \in \Lambda \big \rangle
                \land 
            \big \langle \lambda \in \Delta \big \rangle
        \Big]
    \end{equation*}
    By DeMorgans law (from logic), 
    and by the definitions for set membership and set complementation, that is 
    \begin{equation*}
        \lnot \Big \langle \lambda \in \mathrm{A} \Big \rangle 
            \lor 
        \lnot \Big \langle \lambda \in \Lambda \Big \rangle 
            \lor 
        \lnot \Big \langle \lambda \in \Delta \Big \rangle
            \equiv
        \Big \langle \lambda \in \overline{\mathrm{A}} \Big \rangle 
            \lor 
        \Big \langle \lambda \in \overline{\Lambda} \Big \rangle
            \lor 
        \Big \langle \lambda \in \overline{\Delta} \Big \rangle
    \end{equation*}
    $\therefore \text{\space} \bm{
    \overline{
            \mathrm{A} 
                \cap 
            \Lambda 
                \cap 
            \Delta
    } 
        = 
    \overline{\mathrm{A}} 
        \cup 
    \overline{\Lambda} 
        \cup 
    \overline {\Delta}}
    $,
    by the definition for the union of sets.
\color{lightgray} \end{proof}

\end{document}