\documentclass[preview]{standalone}
\usepackage{amssymb, amsthm}
\usepackage{mathtools}
\usepackage{bm}


\newtheorem{theorem}{Theorem}
\renewcommand\qedsymbol{$\blacksquare$}


\begin{document}


\begin{theorem}[\textbf{2346}]
    Let \bm{$\lambda$} be a real number, 
    and let \bm{$\zeta$} be an integer. 
    \begin{equation*}
        \bm{\lceil \lambda + \zeta \rceil 
            =
        \lceil \lambda \rceil + \zeta}
    \end{equation*}
\end{theorem}

\begin{proof}
    Given \bm{$\lceil \lambda \rceil$}, by the properties for ceiling functions we have
    \begin{equation*}
        \Big \langle \lceil \lambda \rceil - 1 \Big \rangle
            < 
        \Big \langle \lambda \Big \rangle
            \le 
        \Big \langle \lceil \lambda \rceil \Big \rangle
    \end{equation*}
    By the additive compatibility law from the order axioms, that is
    \begin{equation*}
        \Big \langle \big[ \lceil \lambda \rceil + \zeta \big] - 1 \Big \rangle
            < 
        \Big \langle \lambda + \zeta \Big \rangle
            \le 
        \Big \langle \lceil \lambda \rceil + \zeta \Big \rangle
    \end{equation*} 
    $\therefore \text{\space} \bm{
    \lceil \lambda + \zeta \rceil = \lceil \lambda \rceil + \zeta$},
    by the properties for ceiling functions.
    
\end{proof}


\end{document}