\documentclass[preview]{standalone}
\usepackage{amssymb, amsthm}
\usepackage{mathtools}
\usepackage{bm}
\usepackage{xcolor}


\newtheorem*{theorem*}{Theorem}
\renewcommand\qedsymbol{$\blacksquare$}


\begin{document}


\begin{theorem*}[\textbf{2224}] \color{black}
    Let \bm{$\mathrm{A}$}, \bm{$\Lambda$}, and \bm{$\Delta$} be sets. 
    \begin{equation*}
        \bm{
            \Big \langle \mathrm{A} - \Lambda \Big \rangle - \Delta 
                = 
            \Big \langle \mathrm{A} - \Delta \Big \rangle 
                - 
            \Big \langle \Lambda - \Delta \Big \rangle
        }
    \end{equation*}
\end{theorem*}
\begin{proof} \color{black}
    Let \bm{$\lambda$} be an element in 
    \bm{$
    \big \langle \mathrm{A} - \Lambda \big \rangle - \Delta 
    $}. 
    By the definition for set difference,
    \begin{equation*}
        \bigg[
            \Big \langle \lambda \in \mathrm{A} \Big \rangle
                \land
            \Big \langle \lambda \notin \Lambda \Big \rangle
        \bigg]
            \land
        \Big \langle \lambda \notin \Delta \Big \rangle
    \end{equation*}
    Note that, by the indentity law for logical disjunction, 
    \bm{$
    \lambda \notin \Lambda
        \equiv 
    \lambda \notin \Lambda
        \lor 
    \bot
    $}.
    And since
    \bm{$
    \lambda \in \Delta
        \equiv 
    \bot
    $},
    by definition,
    it follows that
    \begin{equation*}
        \Big \langle \lambda \notin \Lambda \Big \rangle
            \equiv
        \bigg[
            \Big \langle \lambda \notin \Lambda \Big \rangle
                \lor
            \Big \langle \bot \Big \rangle
        \bigg]
            \equiv
        \bigg[
            \Big \langle \lambda \notin \Lambda \Big \rangle
                \lor
            \Big \langle \lambda \in \Delta \Big \rangle
        \bigg]
    \end{equation*}
    Moreover, by the double negation law of logic, and by DeMorgans laws,
    \begin{equation*}
        \Big \langle \lambda \notin \Lambda \Big \rangle
            \equiv
        \lnot \Bigg\{
            \lnot \bigg[
                \Big \langle \lambda \notin \Lambda \Big \rangle
                    \lor
                \Big \langle \lambda \in \Delta \Big \rangle
            \bigg]
        \Bigg\}
            \equiv
        \lnot \bigg[
            \Big \langle \lambda \in \Lambda \Big \rangle
                \land
            \Big \langle \lambda \notin \Delta \Big \rangle
        \bigg]
    \end{equation*}
    Thus, the proposition
    \bm{$
    \lambda \in
    \big \langle \mathrm{A} - \Lambda \big \rangle - \Delta 
    $},
    is equivalent to
    \begin{equation*}
        \Bigg\{
        \Big \langle \lambda \in \mathrm{A} \Big \rangle
            \land
        \lnot \bigg[
            \Big \langle \lambda \in \Lambda \Big \rangle
                \land
            \Big \langle \lambda \notin \Delta \Big \rangle
        \bigg]
        \Bigg\}
            \land
        \Big \langle \lambda \notin \Delta \Big \rangle
    \end{equation*}
    By law of commutativity (and association) for logical conjunction, 
    that is
    \begin{equation*}
        \bigg[
            \Big \langle \lambda \in \mathrm{A} \Big \rangle
                \land
            \Big \langle \lambda \notin \Delta \Big \rangle
        \bigg]
            \land
        \lnot \bigg[
            \Big \langle \lambda \in \Lambda \Big \rangle
                \land
            \Big \langle \lambda \notin \Delta \Big \rangle
        \bigg]
    \end{equation*}
    By the definitions for the difference of sets, set complementation,
    and the intersection of sets,
    \begin{equation*}
        \bigg[
        \Big \langle \mathrm{A} - \Lambda \Big \rangle - \Delta
        \bigg]
            \equiv
        \bigg[
        \Big \langle \mathrm{A} - \Delta \Big \rangle
            \cap
        \overline{
            \Big \langle \Lambda - \Delta \Big \rangle
        }
        \bigg]
    \end{equation*}
    $\therefore \text{\space} \bm{
    \big \langle \mathrm{A} - \Lambda \big \rangle - \Delta 
        = 
    \big \langle \mathrm{A} - \Delta \big \rangle 
        - 
    \big \langle \Lambda - \Delta \big \rangle
    }$, by Thereom 2.2.19

\color{lightgray} \end{proof}

\end{document}