\documentclass[preview]{standalone}
\usepackage{amssymb, amsthm}
\usepackage{mathtools}
\usepackage{bm}
\usepackage{xcolor}


\newtheorem*{theorem*}{Theorem}
\renewcommand\qedsymbol{$\blacksquare$}


\begin{document}


\begin{theorem*}[\textbf{2370e}]
    Let \bm{$\lambda$}, and \bm{$\iota$} be real numbers.
    \begin{equation*}
        \bm{
            \big \lfloor \lambda \rfloor 
                + 
            \big \lfloor \iota \rfloor  
                + 
            \big \lfloor \lambda + \iota \rfloor 
                \le 
            \big \lfloor 2 \lambda \rfloor 
                + 
            \big \lfloor 2 \iota \rfloor
        }
    \end{equation*}
\end{theorem*}

\begin{proof}
    By cases.
    There exist real numbers \bm{$\epsilon$} and \bm{$\sigma$} such that
    \bm{$\lambda - \lfloor \lambda \rfloor = \epsilon$}. 
    By the property for floor functions,
    \bm{$\lfloor \lambda \rfloor = \lambda - \epsilon$},
    if and only if
    \begin{equation*}
        \Big \langle \lambda - \epsilon \Big \rangle
            \leq 
        \Big \langle \lambda \Big \rangle
            < 
        \Big \langle \lambda - \epsilon + 1 \Big \rangle
    \end{equation*}
    Without loss of generality with respect to \bm{$\iota$}, 
    by the additive compatibility law from the order axioms,
    there exists an integer 
    \bm{$
        \lfloor \lambda + \iota \rfloor 
            = 
        \big \langle \lambda - \epsilon \big \rangle
            +
        \big \langle \iota - \sigma \big \rangle$},
    if and only if
    \begin{equation*}
        \Big \langle
            \lambda - \epsilon
                + 
            \iota - \sigma
        \Big \rangle
            \leq 
        \Big \langle \lambda + \iota \Big \rangle
            < 
        \Big \langle
            \lambda - \epsilon
                + 
            \iota - \sigma
                + 
            1
        \Big \rangle
    \end{equation*}
    Thus, by the identities for the floor of \bm{$\lambda$},
    the floor of \bm{$\iota$}, 
    and the floor of the sum of \bm{$\lambda$} and \bm{$\iota$},
    we deduce 
    \begin{equation*}
        \big \lfloor \lambda \big \rfloor
            +
        \big \lfloor \iota \big \rfloor
            +
        \big \lfloor \lambda + \iota \big \rfloor
            =
        \Big[
            \big \langle \lambda - \epsilon \big \rangle
                +
            \big \langle \iota - \sigma \big \rangle
                +
            \big \langle \lambda - \epsilon + \iota - \sigma \big \rangle
        \Big]
            =
    \end{equation*}
    \begin{equation*}
        2 \big \langle \lambda + \iota \big \rangle 
            -
        2 \big \langle \epsilon + \sigma \big \rangle
    \end{equation*}
    Now, by multiplicative compatibility, 
    and transitivity from the order axioms,
    \begin{equation*}
        \Big \langle \lambda - \epsilon \Big \rangle
            \leq 
        \Big \langle \lambda \Big \rangle
            < 
        \Big \langle \lambda - \epsilon + 1 \Big \rangle
            \equiv
        \Big \langle 2 \lambda - 2\epsilon \Big \rangle
            \leq 
        \Big \langle 2 \lambda \Big \rangle
            < 
        \Big \langle 2 \lambda - 2\epsilon + 2 \Big \rangle
            \equiv
    \end{equation*}
    \begin{equation*}
        \Big \langle 2 \big[ \lambda - \epsilon \big] \Big \rangle
            \leq
        \Big \langle 2 \lambda \Big \rangle
            \leq
        \Big \langle 2 \big[ \lambda - \epsilon \big] + 1 \Big \rangle
    \end{equation*}
    So \bm{$
        \big \lfloor 2 \lambda \big \rfloor
    $}
    is the integer
    $(i)$ \bm{$
        2 \big \langle \lambda - \epsilon \big \rangle
    $}, 
    or $(ii)$ \bm{$
        2 \big \langle \lambda - \epsilon \big \rangle + 1
    $}, by the properties for the floor function.
    \\ \\
    \bm{$(i)$} Let \bm{$
        \big \lfloor 2 \lambda \big \rfloor 
            = 
        2 \big \langle \lambda - \epsilon \big \rangle
    $}. 
    Without loss of generality with respect to \bm{$\iota$},
    \begin{equation*}
        \Big \{ 
            \big \lfloor 2 \lambda \big \rfloor 
                + 
            \big \lfloor 2 \iota \big \rfloor
        \Big \}
            =
        \Big \{
            2 \big \langle \lambda - \epsilon \big \rangle 
                + 
            2 \big \langle \iota - \sigma \big \rangle
        \Big \}
            =
        \Big \{
            2 \big \langle \lambda + \iota \big \rangle
                - 
            2 \big \langle \epsilon + \sigma \big \rangle
        \Big \}
            =
    \end{equation*}
    \begin{equation*}
        \Big \{
            \big \lfloor \lambda \big \rfloor
                +
            \big \lfloor \iota \big \rfloor
                +
            \big \lfloor \lambda + \iota \big \rfloor
        \Big \}
    \end{equation*}
    \bm{$(ii)$} Let \bm{$
    \big \lfloor 2 \lambda \big \rfloor
        = 
    2 \big \langle \lambda - \epsilon \big \rangle + 1
    $}.
    Without loss of generality with respect to \bm{$\iota$},
    \begin{equation*}
        \Big \{
            \big \lfloor 2 \lambda \big \rfloor 
                + 
            \big \lfloor 2 \iota \big \rfloor
        \Big \}
            =
        \Big \{
            2 \big \langle \lambda - \epsilon \big \rangle + 1 
                + 
            2 \big \langle \iota - \sigma \big \rangle + 1
        \Big \}
            =
        \Big \{
            2 \big \langle \lambda + \iota + 1 \big \rangle 
                - 
            2 \big \langle \epsilon + \sigma \big \rangle
        \Big \}
    \end{equation*}
    \begin{equation*}
            >
        \Big\{
            \big \lfloor \lambda \big \rfloor
                +
            \big \lfloor \iota \big \rfloor
                +
            \big \lfloor \lambda + \iota \big \rfloor
        \Big\}
    \end{equation*}
    $\therefore \text{\space} \bm{
        \big \lfloor \lambda \rfloor 
            + 
        \big \lfloor \iota \rfloor  
            + 
        \big \lfloor \lambda + \iota \rfloor 
            \le 
        \big \lfloor 2 \lambda \rfloor 
            + 
        \big \lfloor 2 \iota \rfloor 
    }$.
\color{lightgray} \end{proof}

\end{document}